src/verification/semantics/skip_stream.lean
@@ -1,109 +1,345 @@
-import verification.semantics.stream_props
+import tactic.linarith
+import finsupp_lemmas
+import verification.misc
 
-noncomputable theory
 open_locale classical
+noncomputable theory
 
--- skip s i : if current index < i, must advance; may advance to first ready index ≥ i.
--- succ s i : if current index ≤ i, must advance; may advance to first ready index > i.
+universes u
+
+structure Stream (ι : Type) (α : Type u) : Type (max 1 u) :=
+(σ : Type)
+(valid : σ → Prop)
+(ready : σ → Prop)
+(skip  : Π x, valid x → ι ×ₗ bool → σ)
+(index : Π (x : σ), valid x → ι)
+(value : Π (x : σ), ready x → α)
+
+@[ext]
+lemma Stream.ext {ι α} {s₁ s₂ : Stream ι α} (h₀ : s₁.σ = s₂.σ)
+  (h₁ : ∀ x y, x == y → (s₁.valid x ↔ s₂.valid y)) (h₂ : ∀ x y, x == y → (s₁.ready x ↔ s₂.ready y)) (h₃ : ∀ x y H₁ H₂ i, x == y → s₁.skip x H₁ i == s₂.skip y H₂ i)
+  (h₄ : ∀ x y H₁ H₂, x == y → s₁.index x H₁ == s₂.index y H₂) (h₅ : ∀ x y H₁ H₂, x == y → s₁.value x H₁ == s₂.value y H₂) :  s₁ = s₂ :=
+begin
+  cases s₁ with σ₁ v₁ r₁ n₁ i₁ l₁, cases s₂ with σ₂ v₂ r₂ n₂ i₂ l₂, dsimp only at *,
+  subst h₀, simp only [heq_iff_eq] at *,
+  obtain rfl : v₁ = v₂ := funext (λ x, propext $ h₁ x x rfl), obtain rfl : r₁ = r₂ := funext (λ x, propext $ h₂ x x rfl),
+  refine ⟨rfl, rfl, rfl, _, _, _⟩; try { simp only [heq_iff_eq] at * }; ext, { apply h₃ x x _ _ _ rfl; assumption, }, { apply h₄ x x _ _ rfl; assumption, },
+  { apply h₅ x x _ _ rfl; assumption, },
+end
+
+
+section stream_defs
+variables {ι : Type} {α : Type*}
+
+def Stream.eval₀ [has_zero α] (s : Stream ι α) (σ₀ : s.σ) (h₁ : s.valid σ₀) : ι →₀ α :=
+if h₂ : s.ready σ₀ then finsupp.single (s.index _ h₁) (s.value _ h₂) else 0
+
+@[reducible]
+def stream_order (ι : Type) : Type := ι ×ₗ bool
+
+@[simps]
+def Stream.to_order (s : Stream ι α) (q : s.σ) (h : s.valid q) : stream_order ι :=
+(s.index q h, s.ready q)
+
+def Stream.to_order' (s : Stream ι α) (q : s.σ) : (with_top ι) ×ₗ bool :=
+if h : s.valid q then (↑(s.to_order q h).1, (s.to_order q h).2)  else (⊤, ff)
+
+def Stream.index' (s : Stream ι α) (x : s.σ) : with_top ι :=
+if h : s.valid x then s.index x h else ⊤ 
+
+def Stream.value' [has_zero α] (s : Stream ι α) (x : s.σ) : α :=
+if h : s.ready x then s.value _ h else 0
+
+def Stream.next (s : Stream ι α) (q : s.σ) : s.σ :=
+if h : s.valid q then s.skip q h (s.to_order q h) else q
+
+def Stream.skip' (s : Stream ι α) (q : s.σ) (i : ι ×ₗ bool) : s.σ :=
+if h : s.valid q then s.skip q h i else q 
+
+abbreviation coe_lex (x : stream_order ι) : (with_top ι) ×ₗ bool := (↑x.1, x.2)
+
+@[simp] lemma coe_lex_le_iff [preorder ι] {x y : stream_order ι} :
+  coe_lex x ≤ coe_lex y ↔ x ≤ y := by simp [prod.lex.le_iff']
+
+@[simp] lemma coe_lex_lt_iff [preorder ι] {x y : stream_order ι} :
+  coe_lex x < coe_lex y ↔ x < y := by simp [prod.lex.lt_iff']
+
+lemma coe_lex_injective : function.injective (@coe_lex ι)
+| ⟨x₁, y₁⟩ ⟨x₂, y₂⟩ := by simpa using and.intro
+
+@[simp] lemma coe_lex_inj (x y : stream_order ι) : coe_lex x = coe_lex y ↔ x = y :=
+coe_lex_injective.eq_iff
+
+@[simp] lemma Stream.index'_val {s : Stream ι α} {x : s.σ} (h : s.valid x) : s.index' x = s.index x h := dif_pos h
+
+@[simp] lemma Stream.index'_invalid {s : Stream ι α} {x : s.σ} (h : ¬s.valid x) : s.index' x = ⊤ := dif_neg h
+
+@[simp] lemma Stream.value'_val [has_zero α] {s : Stream ι α} {x : s.σ} (h : s.ready x) : s.value' x = s.value x h := dif_pos h
+
+@[simp] lemma Stream.next_val {s : Stream ι α} {x : s.σ} (h : s.valid x) : s.next x = s.skip x h (s.to_order x h) := dif_pos h
+
+@[simp] lemma Stream.next_invalid {s : Stream ι α} {x : s.σ} (h : ¬s.valid x) : s.next x = x := dif_neg h
+
+@[simp] lemma Stream.to_order'_fst (s : Stream ι α) (q : s.σ) :
+  (s.to_order' q).1 = s.index' q := by simp [Stream.to_order', Stream.index', apply_dite prod.fst]
+
+@[simp] lemma Stream.skip'_val {s : Stream ι α} {q : s.σ} (hq : s.valid q) (i : ι ×ₗ bool) :
+  s.skip' q i = s.skip q hq i := dif_pos hq
+
+@[simp] lemma Stream.skip'_invalid {s : Stream ι α} {q : s.σ} (hq : ¬s.valid q) (i : ι ×ₗ bool) :
+  s.skip' q i = q := dif_neg hq
+
+lemma Stream.to_order'_val {s : Stream ι α} {q : s.σ} (hq : s.valid q) :
+  s.to_order' q = (s.index' q, s.ready q) := by simp [Stream.to_order', hq]
+
+@[simp] lemma Stream.coe_lex_to_order {s : Stream ι α} {q : s.σ} (hq : s.valid q) :
+  coe_lex (s.to_order q hq) = s.to_order' q := by simp [Stream.to_order'_val, hq]
+
+@[simp] lemma Stream.to_order'_val_snd {s : Stream ι α} {q : s.σ} (hq : s.valid q) :
+  (s.to_order' q).2 = s.ready q := by simp only [Stream.to_order'_val hq]
+
+@[simp] lemma Stream.index'_lt_top_iff [preorder ι] {s : Stream ι α} {q : s.σ} :
+  s.index' q < ⊤ ↔ s.valid q :=
+by { rw [Stream.index'], split_ifs; simpa [with_top.coe_lt_top], }
+
+@[simp] lemma Stream.get_index' [partial_order ι] {s : Stream ι α} {x : s.σ} (h : (s.index' x).is_some) :
+  option.get h = s.index x (by simpa using h) :=
+by { generalize_proofs hq, simp [hq], }
+
+@[simp] noncomputable def Stream.evaln [add_zero_class α] (s : Stream ι α) : ℕ → s.σ → (ι →₀ α)
+| 0 q := 0
+| (n + 1) q := if h₁ : s.valid q then Stream.evaln n (s.next q) + (s.eval₀ _ h₁) else 0 
+
+localized "notation a ` <ₗ `:50 b := @has_lt.lt (stream_order _) _ a b" in streams
+localized "notation a ` ≤ₗ `:50 b := @has_le.le (stream_order _) _ a b" in streams
+
+class is_bounded {ι : Type} {α : Type*} [linear_order ι] (s : Stream ι α) : Prop :=
+(out : ∃ (wf_rel : s.σ → s.σ → Prop), well_founded wf_rel ∧ 
+  (∀ (q hq i), (wf_rel (s.skip q hq i) q) ∨ 
+    ((i <ₗ s.to_order q hq) ∧ (s.skip q hq i) = q)))
+
+variable [linear_order ι]
+
+def Stream.wf_rel (s : Stream ι α) [is_bounded s] : s.σ → s.σ → Prop := ‹is_bounded s›.out.some    
+localized "notation a ` ≺ `:50 b := Stream.wf_rel _ a b" in streams
+lemma Stream.wf (s : Stream ι α) [is_bounded s] : well_founded s.wf_rel := ‹is_bounded s›.out.some_spec.1
+lemma Stream.wf_valid (s : Stream ι α) [is_bounded s] :
+  ∀ (q hq i), ((s.skip q hq i) ≺ q) ∨ ((i <ₗ s.to_order q hq) ∧ (s.skip q hq i) = q) := ‹is_bounded s›.out.some_spec.2
+
+lemma wf_valid_iff {s : Stream ι α} (wf_rel : s.σ → s.σ → Prop) (q hq i) : 
+  (wf_rel (s.skip q hq i) q) ∨ ((i < s.to_order q hq) ∧ (s.skip q hq i) = q) ↔
+  (wf_rel (s.skip' q i) q) ∨ ((coe_lex i < s.to_order' q) ∧ s.skip' q i = q) :=
+by simp only [Stream.skip'_val hq, ← Stream.coe_lex_to_order hq, coe_lex_lt_iff]
+
+lemma is_bounded.mk' {s : Stream ι α} (h : ∃ (wf_rel : s.σ → s.σ → Prop), well_founded wf_rel ∧ 
+  (∀ (q i), wf_rel (s.skip' q i) q ∨ ((coe_lex i < s.to_order' q) ∧ s.skip' q i = q))) : is_bounded s :=
+⟨by { simp only [wf_valid_iff], rcases h with ⟨r, wfr, hr⟩, exact ⟨r, wfr, λ q _ i, hr q i⟩, }⟩
+
+lemma Stream.wf_valid' (s : Stream ι α) [is_bounded s] (q i) :
+  ((s.skip' q i) ≺ q) ∨ ((coe_lex i < s.to_order' q) ∧ s.skip' q i = q) :=
+if hq : s.valid q then by { rw ← wf_valid_iff, exact s.wf_valid q hq i, }
+else by { right, split, { rw prod.lex.lt_iff', left, simpa [hq] using with_top.coe_lt_top _, }, simp [hq], }
+
+lemma Stream.progress (s : Stream ι α) [is_bounded s] {q hq i} (h : s.to_order q hq ≤ i) :
+  (s.skip q hq i) ≺ q :=
+(s.wf_valid q hq i).resolve_right (λ H, absurd H.1 h.not_lt)
+
+lemma Stream.next_wf (s : Stream ι α) [is_bounded s] (q) (hq : s.valid q) : (s.next q) ≺ q :=
+by { rw [Stream.next_val hq], refine s.progress (le_of_eq _), simp [Stream.to_order, hq], }
+
+lemma Stream.no_backward (s : Stream ι α) [is_bounded s] (q hq i) : 
+  ((s.skip q hq i) ≺ q) ∨ ((s.skip q hq i) = q) :=
+(s.wf_valid q hq i).imp_right and.right
+
+noncomputable def Stream.eval [add_zero_class α] (s : Stream ι α) [is_bounded s] : s.σ → ι →₀ α
+| q := 
+  if h : s.valid q then
+    have s.wf_rel (s.next q) q, from s.next_wf _ h,
+    s.eval₀ q h + Stream.eval (s.next q) 
+  else 0
+  using_well_founded {rel_tac := λ _ _, `[exact ⟨_, s.wf⟩], dec_tac := `[assumption]}
+
+@[simp] lemma Stream.eval_invalid [add_zero_class α] (s : Stream ι α) [is_bounded s] (q : s.σ) (h : ¬s.valid q) :
+  s.eval q = 0 :=
+by rwa [Stream.eval, dif_neg]
+
+@[simp] lemma Stream.eval_valid [add_zero_class α] (s : Stream ι α) [is_bounded s] (q : s.σ) (h : s.valid q) :
+  s.eval q = s.eval₀ q h + s.eval (s.next q) :=
+by rw [Stream.eval, dif_pos]
+
+lemma Stream.eval₀_support [has_zero α] (s : Stream ι α) (x : s.σ) (h : s.valid x) :
+  (s.eval₀ x h).support ⊆ {s.index x h} :=
+by { rw Stream.eval₀, split_ifs, { exact finsupp.support_single_subset, }, simp, }
+
+lemma Stream.eval₀_support' [has_zero α] (s : Stream ι α) {x : s.σ} (h₁ : s.valid x) {i : ι}
+  (h₂ : s.eval₀ x h₁ i ≠ 0) : s.to_order x h₁ = (i, tt) :=
+begin
+  obtain rfl := finset.eq_of_mem_singleton (s.eval₀_support x h₁ (finsupp.mem_support_iff.mpr h₂)),
+  rw [Stream.eval₀] at h₂, split_ifs at h₂ with hr,
+  { simpa [Stream.to_order, Stream.index'_val h₁], }, { simpa using h₂, }
+end
+
+def Stream.is_monotonic (s : Stream ι α) : Prop :=
+∀ q hq i, s.index' q ≤ s.index' (s.skip q hq i)
+
+section mono
+
+lemma Stream.is_monotonic.index_le_index_next {s : Stream ι α} (h : s.is_monotonic) (q : s.σ) :
+  s.index' q ≤ s.index' (s.next q) :=
+begin
+  by_cases H : s.valid q, swap, { simp [H], },
+  simp only [Stream.next, H, dif_pos],
+  apply h,
+end
+
+lemma Stream.is_monotonic.index_le_of_mem_support [add_zero_class α] {s : Stream ι α} [is_bounded s] (hs : s.is_monotonic) {q : s.σ} :
+  ∀ (i : ι), s.eval q i ≠ 0 → s.index' q ≤ i :=
+begin
+  simp only [← finsupp.mem_support_iff], refine well_founded.induction s.wf q _,
+  intros q ih i hi,
+  by_cases H : s.valid q, swap, { exfalso, simpa [H] using hi, },
+  rw [s.eval_valid _ H] at hi,
+  cases finset.mem_union.mp (finsupp.support_add hi) with hi hi,
+  { rw finset.mem_singleton.mp (s.eval₀_support _ H hi), exact (le_of_eq (Stream.index'_val _)), },
+  exact trans (hs.index_le_index_next q) (ih (s.next q) (s.next_wf _ H) i hi),
+end
+
+lemma Stream.is_monotonic.eq_zero_of_lt_index [add_zero_class α] {s : Stream ι α} [is_bounded s] (hs : s.is_monotonic) {q : s.σ} (i : ι) :
+  ↑i < s.index' q → s.eval q i = 0 := by { contrapose!, exact hs.index_le_of_mem_support i, }
+
+
+def Stream.is_strict_mono (s : Stream ι α) : Prop :=
+s.is_monotonic ∧ ∀ (q hq i), s.to_order q hq ≤ i → s.ready q → s.index' q ≠ s.index' (s.skip q hq i)
+
+lemma Stream.is_strict_mono.lt {s : Stream ι α} (hs : s.is_strict_mono) (q hq i) (H : s.to_order q hq ≤ i) (hr : s.ready q) :
+  s.index' q < s.index' (s.skip q hq i) := lt_of_le_of_ne (hs.1 _ _ _) (hs.2 _ _ _ H hr)
+
+lemma Stream.is_strict_mono.next_ne {s : Stream ι α} (hs : s.is_strict_mono)
+  {q : s.σ} (hq : s.valid q) (hr : s.ready q) : s.index' q ≠ s.index' (s.next q) :=
+by { rw [Stream.next_val hq], exact hs.2 q hq _ rfl.le hr, }
+
+lemma Stream.is_strict_mono.spec {s : Stream ι α} (hs : s.is_strict_mono) (q : s.σ) (hv : s.valid q) {i} (hi : s.to_order q hv ≤ i) :
+  s.to_order' q ≤ (s.index' (s.skip q hv i), ff) :=
+prod.lex.le_iff''.mpr ⟨by simpa using (hs.1 q hv i), by { simp, contrapose, simpa [hv] using hs.2 q hv i hi, }⟩
+
+lemma Stream.is_strict_mono.index_le_of_mem_support [add_zero_class α] {s : Stream ι α} [is_bounded s]
+  (hs : s.is_strict_mono) {q : s.σ} (hv) {i} (hi : s.to_order q hv ≤ i) : ∀ (j : ι), s.eval (s.skip q hv i) j ≠ 0 → s.to_order q hv ≤ (j, ff) :=
+λ j hj, coe_lex_le_iff.mp (by { rw [Stream.coe_lex_to_order], refine (hs.spec q hv hi).trans _, simpa using hs.1.index_le_of_mem_support j hj, })
+
+lemma Stream.is_strict_mono.eq_zero_of_lt_index [add_zero_class α] {s : Stream ι α} [is_bounded s]
+  (hs : s.is_strict_mono) {q : s.σ} (hv) {i} (hi : s.to_order q hv ≤ i) (j : ι) : ((j, ff) <ₗ s.to_order q hv) → s.eval (s.skip q hv i) j = 0 :=
+by { contrapose!, exact hs.index_le_of_mem_support hv hi j, }
+
+lemma fst_lt_of_lt_of_lt {α : Type*} [preorder α] :
+  ∀ {x y z : α ×ₗ bool}, x < y → y < z → x.1 < z.1
+| x y ⟨z, ff⟩ h₁ h₂ := prod.lex.fst_lt_of_lt_of_le (h₁.trans h₂) (by simp)
+| x ⟨y, tt⟩ ⟨z, tt⟩ h₁ h₂ := lt_of_le_of_lt (show x.1 ≤ y, from prod.lex.fst_le_of_le h₁.le) (by simpa using h₂)
+| x ⟨y, ff⟩ ⟨z, tt⟩ h₁ h₂ := lt_of_lt_of_le (show x.1 < y, from prod.lex.fst_lt_of_lt_of_le h₁ (by simp)) (prod.lex.fst_le_of_le h₂.le)
+
+lemma Stream.is_strict_mono.eval_skip_eq_zero [add_zero_class α] {s : Stream ι α} [is_bounded s] (hs : s.is_strict_mono) {q : s.σ} (hv : s.valid q) {i : stream_order ι} {j : ι}
+  (h₁ : (j, ff) <ₗ i) (h₂ : i ≤ₗ s.to_order q hv) :
+  s.eval (s.skip q hv i) j = 0 :=
+begin
+  cases eq_or_lt_of_le h₂ with h₂ h₂,
+  { refine hs.eq_zero_of_lt_index _ h₂.symm.le _ _, rwa ← h₂, },
+  { apply hs.1.eq_zero_of_lt_index, refine lt_of_lt_of_le _ (hs.1 _ _ _), rw [Stream.index'_val hv, with_top.coe_lt_coe], exact fst_lt_of_lt_of_lt h₁ h₂, }
+end
+
+lemma Stream.is_strict_mono.eval₀_eq_eval_filter [add_comm_monoid α] {s : Stream ι α} [is_bounded s] (hs : s.is_strict_mono) (q : s.σ) (hv : s.valid q) :
+  s.eval₀ q hv = (s.eval q).filter (λ i, (i, ff) <ₗ s.to_order q hv) :=
+begin
+  rw [s.eval_valid _ hv, finsupp.filter_add],
+  convert (add_zero _).symm,
+  { rw [finsupp.filter_eq_self_iff], intros i hi, rw s.eval₀_support' hv hi, simp, },
+  { rw [finsupp.filter_eq_zero_iff], intros i hi, rw [Stream.next_val hv], refine hs.eq_zero_of_lt_index hv rfl.le i hi, },
+end
+
+end mono
+
+class is_lawful {ι : Type} {α : Type*} [linear_order ι] [add_zero_class α] (s : Stream ι α) extends is_bounded s :=
+(mono : s.is_monotonic)
+(skip_spec : ∀ q hq i j, (i ≤ₗ (j, ff)) → s.eval (s.skip q hq i) j = s.eval q j)
+
+class is_strict_lawful {ι : Type} {α : Type*} [linear_order ι] [add_zero_class α] (s : Stream ι α) extends is_lawful s :=
+(strict_mono : s.is_strict_mono)
+
+variables [add_zero_class α]
+
+lemma Stream.mono (s : Stream ι α) [is_lawful s] : s.is_monotonic :=
+‹is_lawful s›.mono
+
+lemma Stream.strict_mono (s : Stream ι α) [is_strict_lawful s] : s.is_strict_mono :=
+‹is_strict_lawful s›.strict_mono
+
+lemma Stream.skip_spec (s : Stream ι α) [is_lawful s] (q : s.σ) (hq : s.valid q) (i : stream_order ι) : 
+  (s.eval (s.skip q hq i)).filter (λ j, i ≤ₗ (j, ff)) = (s.eval q).filter (λ j, i ≤ₗ (j, ff)) :=
+by { rw finsupp.filter_ext_iff, exact is_lawful.skip_spec q hq i, }
+
+lemma Stream.skip_lt_to_order {s : Stream ι α} [is_lawful s] {q : s.σ} {hq : s.valid q}
+  {i : stream_order ι} (hi : i < s.to_order q hq) :
+  s.eval (s.skip q hq i) = s.eval q :=
+begin
+  ext j,
+  by_cases H : s.to_order q hq ≤ (j, tt),
+  { rw is_lawful.skip_spec q hq, simpa [prod.lex.lt_iff'', prod.lex.le_iff''] using lt_of_lt_of_le hi H, },
+  have : ↑j < s.index' q := by simpa [hq] using fst_lt_of_lt_of_lt (show (j, ff) <ₗ (j, tt), by simp) (not_le.mp H),
+  rw [s.mono.eq_zero_of_lt_index j this, s.mono.eq_zero_of_lt_index _ (this.trans_le (s.mono q hq i))],
+end
+
+lemma Stream.skip'_lt_to_order {s : Stream ι α} [is_lawful s] {q : s.σ}
+  {i : stream_order ι} (hi : coe_lex i < s.to_order' q) :
+  s.eval (s.skip' q i) = s.eval q :=
+begin
+  by_cases hq : s.valid q, swap, { rw [Stream.skip'_invalid hq], },
+  rw [← Stream.coe_lex_to_order hq, coe_lex_lt_iff] at hi,
+  rw [Stream.skip'_val hq, Stream.skip_lt_to_order hi],
+end
+
+section sanity_check
+
+-- def Stream.denseVec {n : ℕ} (vals : vector α n) : BoundedStream (fin n) α :=
+-- { σ := fin (n + 1),
+--   valid := λ i, ↑i < n,
+--   ready := λ i, ↑i < n,
+--   skip := λ i hi j b, max i (cond b j.succ ↑j),
+--   index := λ i hi, i.cast_lt hi,
+--   value := λ i hi, vals.nth (i.cast_lt hi),
+--   wf_rel := (>),
+--   wf := finite.preorder.well_founded_gt,
+--   wf_valid := λ (i : fin (n + 1)) (hi : ↑i < n) (j : fin n) (b : bool), begin
+--     simp [Stream.to_order, hi],
+--     cases b, { rw prod.lex.lt_iff'', simp, norm_cast, sorry, },
+--     simp, sorry,
+--   end }
+
+
+
+end sanity_check
 
 /-
-if current index < (i, b), must advance; may advance up to first ready index ≥ (i, b) 
+(a * b).eval = (a * b).eval₀ + (a * b).next.eval
+             = (a.eval₀ * b.eval₀ or 0) + (a.skip (i, b) * b.skip (i, b)).eval
+             = a.eval₀ * b.eval₀ + (a.skip (i, b)).eval * (b.skip (i, b)).eval
+
+(ia, ir) ≤ (a.next.index, ff)
+(a.eval₀ * b.eval₀) = a.eval|_{(j, ff) < (ia, ir)} * b.eval|{(j, ff) < (ib, ir)}
+(a * b).eval₀ = (a.eval * b.eval)∣_{(i, ff) < to_order}
+
+(a * b).skip (i, b)
+
+a.eval * b.eval = (a.eval * b.eval)|_{(j, ff) < to_order} + (a.eval * b.eval)|_{to_order ≤ (j, ff)}
+                = (a * b).eval₀ + (a.eval * b.eval)|_{to_order ≤ (j, ff)}
+(a.eval * b.eval)|_{(i, b) ≤ (j, ff)} 
+  = a.eval|_{(i, b) ≤ (j, ff)} * b.eval|_{to_order ≤ (i, ff)}
+  = (a.eval (skip (i, b)))|_{(i, b) ≤ (j, ff)} * (b.eval.skip (i, b))|_{(i, b) ≤ (j, ff)}
+  = (a.eval (skip ..) * b.eval (skip ..))|_{(i, b) ≤ (j, ff)}
+  = (a.eval (next ) * (b.eval (next)))
+
+(a + b).eval = (a + b).eval₀ + (a + b).next.eval
+             = a.eval₀|_{(j, ff) < (i, b)} + b.eval₀|_{(j, ff) < (i, b)}
+                + (a.skip (i, b)).eval + (b.skip (i, b)).eval
+
+
 -/
+end stream_defs
 
-/-- Returns the set of `q` that `s` could skip to if the current state is `x` 
-  and it is supposed to skip past `(i, b)` -/
-def skip_set {ι α : Type*} [linear_order ι] (s : Stream ι α) (x : s.σ) (i : ι) (b : bool) : set s.σ :=
-{q | ∃ (n : ℕ), q = (s.next'^[n] x) ∧ (0 < n ↔ s.to_order x ≤ (i, b)) ∧
-      ∀ m, 0 < m → m < n → s.valid (s.next'^[m] x) → s.ready (s.next'^[m] x) → s.index' (s.next'^[m] x) < i}
-
-structure SkipStream (ι α : Type*) [linear_order ι] extends Stream ι α :=
-(skip : Π x, valid x → ι → bool → σ)
-(hskip : ∀ x hx i b, skip x hx i b ∈ skip_set _ x i b)
-
-variables {ι : Type} {α : Type*} [linear_order ι]
-
-@[simp] noncomputable def SkipStream.eval_skip [add_zero_class α] (s : SkipStream ι α) : ℕ → s.σ → (ι →₀ α)
-| 0 q := 0
-| (n + 1) q := if h₁ : s.valid q then (SkipStream.eval_skip n (s.skip q h₁ (s.index q h₁) (s.ready q))) + (s.eval₀ _ h₁) else 0 
-
-/-- The number of steps a stream would skip at index `(i, b)` -/
-noncomputable def SkipStream.nskip (s : SkipStream ι α) (q : s.σ) (h : s.valid q) (i : ι) (b : bool) : ℕ :=
-  (s.hskip q h i b).some
-
-lemma SkipStream.skip_eq (s : SkipStream ι α) (q : s.σ) (h : s.valid q) (i : ι) (b : bool) :
-  s.skip q h i b = (s.next'^[s.nskip q h i b] q) := (s.hskip q h i b).some_spec.1
-
-lemma SkipStream.advance_iff (s : SkipStream ι α) (q : s.σ) (h : s.valid q) (i : ι) (b : bool) :
-  0 < s.nskip q h i b ↔ s.to_order q ≤ (i, b) := (s.hskip q h i b).some_spec.2.1
-
-/-- All skipped values are less than `i` -/
-lemma SkipStream.lt_of_skipped (s : SkipStream ι α) (q : s.σ) (h : s.valid q) (i : ι) (b : bool)
-  (m : ℕ) (h₁m : 0 < m) (h₂m : m < s.nskip q h i b) (h₃ : s.valid (s.next'^[m] q)) (h₄ : s.ready (s.next'^[m] q)) :
-  s.index' (s.next'^[m] q) < i := (s.hskip q h i b).some_spec.2.2 m h₁m h₂m h₃ h₄
-
-lemma SkipStream.not_ready_of_skipped_of_monotonic (s : SkipStream ι α) (hs : s.monotonic) (q : s.σ) (h : s.valid q) (b : bool)
-  (m : ℕ) (h₁m : 0 < m) (h₂m : m < s.nskip q h (s.index q h) b) (h₃ : s.valid (s.next'^[m] q)) :
-  ¬s.ready (s.next'^[m] q) := λ h₄,
-begin
-  refine (s.lt_of_skipped q h _ b m h₁m h₂m h₃ h₄).not_le _,
-  simpa [Stream.index'_val h] using hs.le_index_iterate q m,
-end
-
-/-- If all skipped states are non-ready, then the eval's are equal -/
-theorem Stream.eval₀_skip_eq [add_comm_monoid α] (s : Stream ι α) (q : s.σ)
-  (n : ℕ) (hn : ∀ m < n, s.valid (s.next'^[m] q) → ¬s.ready (s.next'^[m] q)) :
-  s.eval_steps n q = 0 :=
-begin
-  induction n with n ih generalizing q, { simp, },
-  simp only [Stream.eval_steps, dite_eq_right_iff, forall_true_left],
-  intro h,
-  simp only [Stream.eval₀, (show ¬s.ready q, from hn 0 (nat.zero_lt_succ _) h), dif_neg, not_false_iff, add_zero],
-  apply ih,
-  intros m hm, specialize hn (m + 1) (nat.succ_lt_succ hm),
-  simpa [Stream.next'_val h] using hn,
-end
-
-theorem Stream.eval₀_skip_eq' [add_comm_monoid α] (s : Stream ι α) (q : s.σ) (h : s.valid q)
-  (n : ℕ) (hn : n ≠ 0) (hn : ∀ m, 0 < m → m < n → s.valid (s.next'^[m] q) → ¬s.ready (s.next'^[m] q)) :
-  s.eval_steps n q = s.eval₀ q h :=
-begin
-  cases n, {  contradiction, },
-  have := s.eval₀_skip_eq (s.next q h) n _,
-  { simp [Stream.eval_steps, h, this], },
-  intros m hm,
-  simpa [Stream.next'_val h] using hn (m + 1) m.zero_lt_succ (nat.succ_lt_succ hm),
-end
-
-theorem SkipStream.eval_skip_eq [add_comm_monoid α] (s : SkipStream ι α) (hs : s.monotonic) (q : s.σ) (n : ℕ) :
-  ∃ (m : ℕ), n ≤ m ∧ s.eval_skip n q = s.eval_steps m q :=
-begin
-  induction n with n ih generalizing q, { refine ⟨0, rfl.le, _⟩, simp, },
-  by_cases h : s.valid q, swap,
-  { refine ⟨n + 1, rfl.le, _⟩, simp [h], },
-  rcases ih (s.skip q h (s.index q h) (s.ready q)) with ⟨m, hm₁, hm₂⟩,
-  have : 0 < s.nskip q h (s.index q h) (s.ready q),
-  { rw SkipStream.advance_iff, refine le_of_eq _, ext : 1; simp [Stream.index'_val h], },
-  refine ⟨s.nskip q h (s.index q h) (s.ready q) + m, _, _⟩,
-  { rw nat.succ_le_iff, refine lt_of_le_of_lt hm₁ _, simpa, },
-  rw [s.eval_steps_add, s.eval₀_skip_eq' q h, ← SkipStream.skip_eq],
-  { simp [h, add_comm, hm₂], }, { rwa ← zero_lt_iff, },
-  exact s.not_ready_of_skipped_of_monotonic hs q h _,
-end
-
-lemma SkipStream.eval_skip_eq_of_bounded [add_comm_monoid α] (s : SkipStream ι α) (hs : s.monotonic) (q : s.σ)
-  {B : ℕ} (hB : s.bound_valid B q) : s.eval_skip B q = s.eval_steps B q :=
-by { obtain ⟨m, hm₁, hm₂⟩ := s.eval_skip_eq hs q B, rw [hm₂, Stream.eval_ge_bound hB hm₁], } 
-
-/-- `next` is always a valid skip function -/
-def Stream.default_skip (s : Stream ι α) (q : s.σ) (hq : s.valid q)
-  (i : ι) (b : bool) : s.σ :=
-if s.to_order q ≤ (i, b) then s.next q hq
-else q
-
-lemma Stream.default_skip_valid (s : Stream ι α) (q : s.σ) (hq : s.valid q)
-  (i : ι) (b : bool) : s.default_skip q hq i b ∈ skip_set s q i b :=
-begin
-  rw [Stream.default_skip], split_ifs with H,
-  { exact ⟨1, by simp [hq], by simpa, λ m hm₁ hm₂, (ne_of_lt hm₁ (nat.lt_one_iff.mp hm₂).symm).elim⟩, },
-  { exact ⟨0, rfl, by simpa using H, by simp⟩, }
-end
