src/verification/semantics/stream_add.lean
@@ -1,262 +1,165 @@
-import verification.semantics.stream_props
-import verification.semantics.stream_zero
-import verification.misc
-import verification.semantics.finsuppeval
-import tactic.zify
-import tactic.linarith
-import tactic.abel
+import verification.semantics.skip_stream
 
-open_locale classical
 noncomputable theory
+open_locale streams
+variables {ι : Type} [linear_order ι] {α : Type*}
 
-variables {ι : Type} {α : Type*}
-  [linear_order ι]
-
-section defs
-variables [has_zero α]
-  [has_add α]
-
-@[simps]
-instance : has_add (Stream ι α) := ⟨λ a b,
+@[simps] def Stream.add [has_zero α] [has_add α] (a b : Stream ι α) : Stream ι α :=
 { σ := a.σ × b.σ,
   valid := λ s, a.valid s.1 ∨ b.valid s.2,
-  ready := λ s, (a.to_order s.1 ≤ b.to_order s.2 ∧ a.ready s.1) ∨ (b.to_order s.2 ≤ a.to_order s.1 ∧ b.ready s.2),
-  next := λ s h, (if H : a.to_order s.1 ≤ b.to_order s.2 then a.next s.1 (valid_of_le_or h H) else s.1, 
-                  if H : b.to_order s.2 ≤ a.to_order s.1 then b.next s.2 (valid_of_le_or h.symm H) else s.2),
+  ready := λ s, (a.to_order' s.1 ≤ b.to_order' s.2 ∧ a.ready s.1) ∨ (b.to_order' s.2 ≤ a.to_order' s.1 ∧ b.ready s.2),
+  skip := λ p hp i, (a.skip' p.1 i, b.skip' p.2 i),
   index := λ s h, option.get (show (min (a.index' s.1) (b.index' s.2)).is_some, by simpa),
-  value := λ s h, (if a.to_order s.1 ≤ b.to_order s.2 then a.value' s.1 else 0) +
-                  (if b.to_order s.2 ≤ a.to_order s.1 then b.value' s.2 else 0) }⟩ 
-
--- Some weird inequality lemma I extracted from the main proof
-private lemma succ_le_min_succ_add_succ {a b b' d : ℕ} (ha : a ≤ b + d) (hb' : b ≤ b') :
-  a + 1 ≤ (min b' (b + 1)) + (d + 1) :=
-by { rw [← add_assoc, nat.succ_le_succ_iff, min_def], split_ifs; linarith, }
-
-end defs
-
-section lemmas
-variables {a : Stream ι α} {b : Stream ι α} {x : a.σ} {y : b.σ}
+  value := λ s h, (if a.to_order' s.1 ≤ b.to_order' s.2 then a.value' s.1 else 0) +
+                  (if b.to_order' s.2 ≤ a.to_order' s.1 then b.value' s.2 else 0) } 
 
 section index_lemmas
 variables [has_zero α] [has_add α]
 
-lemma lt_index_of_valid (h : a.to_order x ≤ b.to_order y) (hva : a.valid x) :
-  ↑(a.index x hva) ≤ b.index' y :=
-by { simp only [← Stream.index'_val hva], exact prod.lex.fst_le_of_le h, }
+-- lemma to_order_of_a_invalid {a b : Stream ι α} {q : (a.add b).σ} (ha : ¬a.valid q.1) 
+--   (hq : (a.add b).valid q) : (a.add b).to_order q hq = b.to_order q.2 (hq.resolve_left ha) :=
+-- begin
+--   have : b.to_order' q.2 < a.to_order' q.1,
+--   { rw prod.lex.lt_iff', left, simpa [ha] using hq.resolve_left ha, },
+--   simp [Stream.to_order, ha, this.le, this.not_le],
+-- end
 
-lemma Stream.min_index (h : a.to_order x ≤ b.to_order y) (hva : a.valid x) :
-  min (a.index' x) (b.index' y) = a.index x hva :=
-by { rw [Stream.index'_val hva, min_eq_left_iff], exact lt_index_of_valid h hva, }
+-- lemma to_order_of_b_invalid {a b : Stream ι α} {q : (a.add b).σ} (hb : ¬b.valid q.2) 
+--   (hq : (a.add b).valid q) : (a.add b).to_order q hq = a.to_order q.1 (hq.resolve_right hb) :=
+-- begin
+--   have : a.to_order' q.1 < b.to_order' q.2,
+--   { rw prod.lex.lt_iff', left, simpa [hb] using hq.resolve_right hb, },
+--   simp [Stream.to_order, hb, this.le, this.not_le],
+-- end
 
-@[simp] lemma Stream.add_index' (a : Stream ι α) (b : Stream ι α) (xy : a.σ × b.σ) :
-  (a + b).index' xy = min (a.index' xy.1) (b.index' xy.2) :=
+@[simp] lemma add_index_eq_min {a b : Stream ι α} (q : (a.add b).σ) :
+  (a.add b).index' q = min (a.index' q.1) (b.index' q.2) :=
+by { by_cases H : (a.add b).valid q, { simp [H], }, { simp [H, not_or_distrib.mp H], } }
+
+lemma valid_of_to_order_lt {a b : Stream ι α} {qa : a.σ} {qb : b.σ} (h : a.to_order' qa < b.to_order' qb) :
+  a.valid qa :=
+by { contrapose! h, by_cases hb : b.valid qb, { rw prod.lex.le_iff', left, simpa [h], }, { simp [Stream.to_order', h, hb], } }
+
+@[simp] lemma add_skip_fst {a b : Stream ι α} (q i) : ((a.add b).skip' q i).fst = a.skip' q.1 i :=
+by { simp only [Stream.skip'], split_ifs with h₁ h₂ h₂, { simp [h₂], }, { simp [h₂], }, { cases h₁ (or.inl h₂), }, { refl, }, }
+
+@[simp] lemma add_skip_snd {a b : Stream ι α} (q i) : ((a.add b).skip' q i).snd = b.skip' q.2 i :=
+by { simp only [Stream.skip'], split_ifs with h₁ h₂ h₂, { simp [h₂], }, { simp [h₂], }, { cases h₁ (or.inr h₂), }, { refl, }, }
+
+lemma of_to_order_eq {a b : Stream ι α} (q : (a.add b).σ) (h : a.to_order' q.1 = b.to_order' q.2) :
+  (¬((a.add b).valid q) ∧ ¬(a.valid q.1) ∧ ¬(b.valid q.2)) ∨
+  ((a.add b).valid q ∧ a.valid q.1 ∧ b.valid q.2 ∧ (a.ready q.1 ↔ b.ready q.2) ∧ a.index' q.1 = b.index' q.2) :=
 begin
-  rcases xy with ⟨x, y⟩,
-  by_cases H : (a + b).valid (x, y),
-  { simp [Stream.index'_val H], },
-  { have : ¬a.valid x ∧ ¬b.valid y := by { simpa [not_or_distrib] using H, },
-    simp [Stream.index', H, this], }
+  have : a.index' q.1 = b.index' q.2 := by simpa using congr_arg prod.fst h,
+  by_cases H : (a.add b).valid q,
+  { right, 
+    obtain ⟨hv₁, hv₂⟩ : a.valid q.1 ∧ b.valid q.2, { simp only [← Stream.index'_lt_top_iff] at H ⊢, simpa [this, -Stream.index'_lt_top_iff] using H, },
+    refine ⟨H, hv₁, hv₂, _, this⟩,
+    simpa [hv₁, hv₂] using congr_arg prod.snd h, },
+  { left, refine ⟨H, not_or_distrib.mp H⟩, },
 end
+
+lemma add_to_order_eq_min {a b : Stream ι α} (q : (a.add b).σ) :
+  (a.add b).to_order' q = min (a.to_order' q.1) (b.to_order' q.2) :=
+begin
+  rcases lt_trichotomy (a.to_order' q.1) (b.to_order' q.2) with (h|h|h),
+  { rw min_eq_left h.le, ext : 1,
+    { simpa using prod.lex.fst_le_of_le h.le, },
+    { simp [valid_of_to_order_lt h, h.le, h.not_le], }, },
+  { rcases of_to_order_eq _ h with (⟨H, hv₁, hv₂⟩|⟨H, hv₁, hv₂, hr, hi⟩),
+    { simp [Stream.to_order', H, hv₁, hv₂], },
+    ext : 1, { simp [h, hi], }, simp [Stream.to_order'_val_snd H, h, Stream.to_order'_val_snd hv₂, hr], },
+  { rw min_eq_right h.le, ext : 1,
+    { simpa using prod.lex.fst_le_of_le h.le, },
+    { simp [valid_of_to_order_lt h, h.le, h.not_le], }, },
+end
+
+lemma add_to_order_left {a b : Stream ι α} {q : (a.add b).σ} (hq hq') (ha : a.to_order' q.1 ≤ b.to_order' q.2) :
+  (a.add b).to_order q hq = a.to_order q.1 hq' :=
+coe_lex_injective (by simpa [add_to_order_eq_min])
+
+lemma add_to_order_right {a b : Stream ι α} {q : (a.add b).σ} (hq hq') (ha : b.to_order' q.2 ≤ a.to_order' q.1) :
+  (a.add b).to_order q hq = b.to_order q.2 hq' :=
+coe_lex_injective (by simpa [add_to_order_eq_min])
+
+instance Stream.add.is_bounded (a b : Stream ι α) [is_bounded a] [is_bounded b] : is_bounded (a.add b) :=
+is_bounded.mk' ⟨prod.rprod_eq a.wf_rel b.wf_rel, prod.rprod_eq_wf a.wf b.wf, λ q i, begin
+  rcases a.wf_valid' q.1 i with (h|⟨ha₁, ha₂⟩),
+  { left, left, simp only [add_skip_fst, add_skip_snd], exact ⟨h, (b.wf_valid' q.2 i).imp_right and.right⟩, },
+  rcases b.wf_valid' q.2 i with (h|⟨hb₁, hb₂⟩),
+  { left, right, simp only [add_skip_fst, add_skip_snd], exact ⟨h, (a.wf_valid' q.1 i).imp_right and.right⟩, },
+  right, split,
+  { rw [add_to_order_eq_min, lt_min_iff], split; assumption, }, { ext; simpa, }
+end⟩
 
 end index_lemmas
 
 section value_lemmas
 variables [add_comm_monoid α]
 
-lemma Stream.add.eval₀_left (h : a.to_order x < b.to_order y) (hva H) :
-  (a + b).eval₀ (x, y) H = a.eval₀ x hva :=
+lemma Stream.add.eval₀_eq_left {a b : Stream ι α} {q : (a.add b).σ} (hq : (a.add b).valid q) (H : a.to_order' q.1 < b.to_order' q.2) :
+  (a.add b).eval₀ q hq = a.eval₀ q.1 (valid_of_to_order_lt H) :=
 begin
-  simp [Stream.eval₀, h.le, h.not_le],
-  split_ifs with H,
-  { simp [Stream.min_index h.le hva, Stream.value'_val H], },
-  { refl, },
+  have := add_to_order_left hq (valid_of_to_order_lt H) H.le,
+  have hr : (a.add b).ready q ↔ a.ready q.1, { simpa using congr_arg prod.snd this, },
+  simp only [Stream.eval₀, ← Stream.value'_val, dite_eq_ite], rw [hr],
+  split_ifs with hr', swap, { refl, },
+  congr' 1, { simpa using congr_arg prod.fst this, },
+  simp [@Stream.value'_val _ _ _ (a.add b) _ (or.inl ⟨H.le, hr'⟩), H.le, H.not_le],
 end
 
-lemma Stream.add_eval₀_right (h : b.to_order y < a.to_order x) (hvb H) :
-  (a + b).eval₀ (x, y) H = b.eval₀ y hvb :=
+lemma Stream.add.eval₀_eq_right {a b : Stream ι α} {q : (a.add b).σ} (hq : (a.add b).valid q) (H : b.to_order' q.2 < a.to_order' q.1) :
+  (a.add b).eval₀ q hq = b.eval₀ q.2 (valid_of_to_order_lt H) :=
 begin
-  simp [Stream.eval₀, h.le, h.not_le],
-  split_ifs with H,
-  { simp [H, Stream.min_index h.le hvb, Stream.value'_val H, min_comm (a.index' _) _], },
-  { refl, },
+  have := add_to_order_right hq (valid_of_to_order_lt H) H.le,
+  have hr : (a.add b).ready q ↔ b.ready q.2, { simpa using congr_arg prod.snd this, },
+  simp only [Stream.eval₀, ← Stream.value'_val, dite_eq_ite], rw [hr],
+  split_ifs with hr', swap, { refl, },
+  congr' 1, { simpa using congr_arg prod.fst this, },
+  simp [@Stream.value'_val _ _ _ (a.add b) _ (or.inr ⟨H.le, hr'⟩), H.le, H.not_le],
 end
 
-lemma Stream.add_eval₀_both (h : a.to_order x = b.to_order y) (hva hvb H) :
-  (a + b).eval₀ (x, y) H = a.eval₀ x hva + b.eval₀ y hvb :=
+lemma Stream.add.eval₀_eq_both {a b : Stream ι α} {q : (a.add b).σ} (hq : (a.add b).valid q) (H : a.to_order' q.1 = b.to_order' q.2) (hv₁ hv₂) (hr : a.ready q.1 ↔ b.ready q.2) 
+  (hi : a.index q.1 hv₁ = b.index q.2 hv₂) : (a.add b).eval₀ q hq = a.eval₀ q.1 hv₁ + b.eval₀ q.2 hv₂ :=
 begin
-  simp [Stream.eval₀, h],
-  have : a.index _ hva = b.index _ hvb, { simpa [Stream.index'_val hva, Stream.index'_val hvb] using congr_arg prod.fst h, },
-  by_cases H₁ : a.ready x; by_cases H₂ : b.ready y; simp [H₁, H₂, Stream.value', Stream.min_index h.le hva, this],
+  have : (a.add b).ready q ↔ b.ready q.2, { simp [H, hr], },
+  simp only [Stream.eval₀, ← Stream.value'_val, dite_eq_ite], rw [this, hr],
+  split_ifs with hr', swap, { simp, },
+  rw [hi, ← finsupp.single_add, Stream.add_index, @Stream.value'_val _ _ _ (a.add b)],
+  { simp [Stream.index'_val hv₁, Stream.index'_val hv₂, hi, -finsupp.single_add, H], },
+  right, refine ⟨_, hr'⟩, rw [H],
+end
+
+lemma Stream.add_spec (a b : Stream ι α) [is_lawful a] [is_lawful b] (q : (a.add b).σ) :
+  (a.add b).eval q = (a.eval q.1) + (b.eval q.2) :=
+begin
+  refine @well_founded.induction _ (a.add b).wf_rel (a.add b).wf _ q _,
+  clear q, intros q ih,
+  rcases lt_trichotomy (a.to_order' q.1) (b.to_order' q.2) with (h|h|h),
+  { have hv : a.valid q.1 := valid_of_to_order_lt h,
+    have hq : (a.add b).valid q := or.inl hv,
+    rw [(a.add b).eval_valid q hq, ih _ ((a.add b).next_wf _ hq), Stream.next_val hq, Stream.add_skip, @Stream.skip'_lt_to_order _ _ _ _ b,
+      add_to_order_left hq hv h.le, Stream.skip'_val hv, a.eval_valid _ hv, add_assoc, Stream.add.eval₀_eq_left hq h, Stream.next_val hv],
+    simpa [add_to_order_eq_min], },
+  { rcases of_to_order_eq _ h with (⟨H, hv₁, hv₂⟩|⟨hq, hv₁, hv₂, hr, hi⟩),
+    { simp [H, hv₁, hv₂], },
+    obtain ⟨t₀, t₁⟩ : (a.add b).to_order q hq = a.to_order q.1 hv₁ ∧ (a.add b).to_order q hq = b.to_order q.2 hv₂,
+    { split; apply_fun coe_lex using coe_lex_injective; simp [add_to_order_eq_min, h], },
+    simp only [Stream.index'_val, hv₁, hv₂, with_top.coe_eq_coe] at hi,
+    rw [(a.add b).eval_valid q hq, ih _ ((a.add b).next_wf _ hq), Stream.next_val hq, Stream.add_skip, Stream.add.eval₀_eq_both hq h hv₁ hv₂ hr hi,
+      (show ∀ (w x y z : ι →₀ α), (w + x) + (y + z) = (w + y) + (x + z), by intros; abel)], dsimp only,
+    congr' 1,
+    { rw [a.eval_valid _ hv₁, Stream.next_val hv₁, t₀, Stream.skip'_val hv₁], },
+    { rw [b.eval_valid _ hv₂, Stream.next_val hv₂, t₁, Stream.skip'_val hv₂], }, },
+  { have hv : b.valid q.2 := valid_of_to_order_lt h,
+    have hq : (a.add b).valid q := or.inr hv,
+    rw [(a.add b).eval_valid q hq, ih _ ((a.add b).next_wf _ hq), Stream.next_val hq, Stream.add_skip, @Stream.skip'_lt_to_order _ _ _ _ a,
+      add_to_order_right hq hv h.le, Stream.skip'_val hv, b.eval_valid _ hv, add_left_comm, Stream.add.eval₀_eq_right hq h, Stream.next_val hv],
+    simpa [add_to_order_eq_min], },
 end
 
 end value_lemmas
-end lemmas
 
-@[elab_as_eliminator]
-theorem Stream.add_induction [has_zero α] [has_add α] (a : Stream ι α) (b : Stream ι α) (x : a.σ) (y : b.σ)
-  {B₁ B₂ : ℕ} (ha : a.bound_valid B₁ x) (hb : b.bound_valid B₂ y)
-  (P : ∀ (x : a.σ) (y : b.σ) (k₁ : ℕ) (k₂ : ℕ) (N : ℕ), Prop)
-  (hP_base : ∀ (x y), P x y 0 0 0)
-  (hP_invalid : ∀ (x y B₁ B₂ N) (H : ¬(a + b).valid (x, y)) (hvx : ¬a.valid x) (hvy : ¬b.valid y), a.bound_valid B₁ x → b.bound_valid B₂ y → P x y B₁ B₂ N)
-  (hP_advance_a : ∀ (x y k₁ k₂ N) (hvx : a.valid x), (a + b).valid (x, y) → a.to_order x < b.to_order y → P (a.next x hvx) y k₁ k₂ N → P x y (k₁ + 1) k₂ (N + 1))
-  (hP_advance_b : ∀ (x y k₁ k₂ N) (hvy : b.valid y), (a + b).valid (x, y) → b.to_order y < a.to_order x → P x (b.next y hvy) k₁ k₂ N → P x y k₁ (k₂ + 1) (N + 1))
-  (hP_advance_both : ∀ (x y k₁ k₂ B₁ N) (hvx : a.valid x) (hvy : b.valid y), (a + b).valid (x, y) → a.bound_valid (B₁ + 1) x → a.to_order x = b.to_order y → P (a.next x hvx) (b.next y hvy) k₁ k₂ N → P x y (min (B₁ + 1) (k₁ + 1)) (k₂ + 1) (N + 1)) :
-  P x y B₁ B₂ (B₁ + B₂) :=
-begin
-  suffices : ∀ n ≤ B₁ + B₂, ∃ (k₁ k₂ : ℕ), k₁ ≤ B₁ ∧ k₂ ≤ B₂ ∧ n ≤ k₁ + k₂ ∧ P x y k₁ k₂ n,
-  { obtain ⟨k₁, k₂, h₁, h₂, hn, hP⟩ := this (B₁ + B₂) rfl.le,
-    obtain ⟨rfl, rfl⟩ : k₁ = B₁ ∧ k₂ = B₂ := by split; linarith only [h₁, h₂, hn],
-    exact hP, },
-  intros n hn,
-  induction n with n ih generalizing B₁ B₂ x y,
-  { use [0, 0], simpa using hP_base x y, },
-  by_cases H : (a + b).valid (x, y), swap,
-  { -- Invalid
-    obtain ⟨hvx, hvy⟩ : ¬a.valid x ∧ ¬b.valid y := by simpa [not_or_distrib] using H,
-    refine ⟨B₁, B₂, rfl.le, rfl.le, hn, _⟩, 
-    exact hP_invalid _ _ _ _ _ H hvx hvy ha hb, },
-  rcases lt_trichotomy (a.to_order x) (b.to_order y) with h|h|h, swap, rotate 1,
-  { -- Advancing `a`
-    have hvx : a.valid x := valid_of_le_or H h.le,
-    cases B₁, { cases hvx.bound_pos ha, },
-    rw [Stream.bound_valid_succ] at ha,
-    obtain ⟨k₁, k₂, hk₁, hk₂, n_le, hP⟩ := ih (a.next _ hvx) y (ha hvx) hb (by simpa [nat.succ_eq_one_add, add_assoc] using hn),
-    refine ⟨k₁ + 1, k₂, nat.succ_le_succ hk₁, hk₂, _, _⟩,
-    { ac_change _ ≤ k₁ + k₂ + 1, exact nat.succ_le_succ n_le, },
-    exact hP_advance_a _ _ _ _ _ hvx H h hP, },
-  { -- Advancing `b`
-    have hvy : b.valid y := valid_of_le_or (or.symm H) h.le,
-    cases B₂, { cases hvy.bound_pos hb, },
-    rw [Stream.bound_valid_succ] at hb,
-    obtain ⟨k₁, k₂, hk₁, hk₂, n_le, hP⟩ := ih x (b.next _ hvy) ha (hb hvy) (nat.le_of_succ_le_succ hn),
-    refine ⟨k₁, k₂ + 1, hk₁, nat.succ_le_succ hk₂, nat.succ_le_succ n_le, _⟩,
-    exact hP_advance_b _ _ _ _ _ hvy H h hP, },
-  { -- Advancing both `a` and `b`
-    have hvx : a.valid x := valid_of_le_or H h.le,
-    have hvy : b.valid y := valid_of_le_or (or.symm H) h.symm.le,
-    cases B₁, { cases hvx.bound_pos ha, },
-    cases B₂, { cases hvy.bound_pos hb, },
-    have ha' := ha, rw nat.succ_eq_add_one at ha',
-    rw [Stream.bound_valid_succ] at ha hb,
-    obtain ⟨k₁, k₂, hk₁, hk₂, n_le, hP⟩ := ih (a.next _ hvx) (b.next _ hvy) ((ha hvx).mono B₁.le_succ) (hb hvy) (nat.le_of_succ_le_succ hn),
-    refine ⟨min (B₁ + 1) (k₁ + 1), k₂ + 1, min_le_left _ _, nat.succ_le_succ hk₂, succ_le_min_succ_add_succ n_le hk₁, _⟩, 
-    exact hP_advance_both _ _ _ _ _ _ hvx hvy H ha' h hP, }
-end
 
-theorem Stream.add_spec [add_comm_monoid α] (a : Stream ι α) (b : Stream ι α) (x : a.σ) (y : b.σ)
-  {B₁ B₂ : ℕ} (ha : a.bound_valid B₁ x) (hb : b.bound_valid B₂ y) :
-  (a + b).eval_steps (B₁ + B₂) (x, y) = a.eval_steps B₁ x + b.eval_steps B₂ y :=
-begin
-  apply Stream.add_induction a b x y ha hb (λ x y k₁ k₂ N, (a + b).eval_steps N (x, y) = a.eval_steps k₁ x + b.eval_steps k₂ y); clear_except,
-  { intros, simp, },
-  { intros x y B₁ B₂ n H hvx hvy ha hb,
-    simp [Stream.eval_invalid H, Stream.eval_invalid hvx, Stream.eval_invalid hvy], },
-  { intros x y k₁ k₂ n hvx H h he,
-    dsimp, simp [h.le, h.not_le, he, Stream.add.eval₀_left h hvx, H, hvx],
-    apply add_right_comm, },
-  { intros x y k₁ k₂ n hvy H h he, 
-    dsimp [nat.add_succ], simp [H, hvy, h.le, h.not_le, he, Stream.add_eval₀_right h hvy, add_assoc], },
-  { intros x y k₁ k₂ B₁ n hvx hvy H ha h he, 
-    rw Stream.eval_min_bound ha,
-    dsimp, simp [h.le, h.symm.le, he, Stream.add_eval₀_both h hvx hvy, H, hvx, hvy],
-    abel, },
-end
-
-theorem Stream.add_spec_index [has_zero α] [has_add α] (a : Stream ι α) (b : Stream ι α) (x : a.σ) (y : b.σ)
-  {B₁ B₂ : ℕ} (ha : a.bound_valid B₁ x) (hb : b.bound_valid B₂ y) :
-  ((a + b).next'^[B₁ + B₂] (x, y)) = (a.next'^[B₁] x, b.next'^[B₂] y) :=
-begin
-  apply Stream.add_induction a b x y ha hb (λ x y k₁ k₂ N, ((a + b).next'^[N] (x, y)) = (a.next'^[k₁] x, b.next'^[k₂] y)); clear_except,
-  { intros, simp, },
-  { intros x y B₁ B₂ n H hvx hvy ha hb, 
-    simp [Stream.next'_val_invalid' H, Stream.next'_val_invalid' hvx, Stream.next'_val_invalid' hvy], },
-  { intros x y k₁ k₂ n hvx H h hiter,
-    simp [Stream.next'_val hvx, Stream.next'_val H, h.le, h.not_le, hiter], },
-  { intros x y k₁ k₂ n hvy H h hiter,
-    simp [Stream.next'_val hvy, Stream.next'_val H, h.le, h.not_le, hiter], },
-  { intros x y k₁ k₂ B₁ n hvx hvy H ha h hiter, 
-    rw Stream.next'_min_bound ha,
-    simp [h.le, h.symm.le, hiter, Stream.next'_val hvx, Stream.next'_val hvy, Stream.next'_val H], }
-end
-
-@[simps]
-instance [has_zero α] [has_add α] : has_add (StreamExec ι α) := ⟨λ a b,
-{ stream := a.stream + b.stream,
-  state := (a.state, b.state),
-  bound := a.bound + b.bound,
-  bound_valid := begin
-    rw [bound_valid_iff_next'_iterate], dsimp,
-    simpa [bound_valid_iff_next'_iterate, (Stream.add_spec_index a.stream b.stream _ _ a.bound_valid b.bound_valid),
-      not_or_distrib] using (and.intro a.bound_valid b.bound_valid),
-  end }⟩
-
-@[simp] lemma StreamExec.add_spec [add_comm_monoid α] (a : StreamExec ι α) (b : StreamExec ι α) :
-  (a + b).eval = a.eval + b.eval := (Stream.add_spec a.stream b.stream _ _ a.bound_valid b.bound_valid)
-
-lemma Stream.add_monotonic [has_zero α] [has_add α] {a : Stream ι α} {b : Stream ι α}
-  (ha : a.monotonic) (hb : b.monotonic) :
-  (a + b).monotonic :=
-begin
-  rintros ⟨x, y⟩ h,
-  simp only [Stream.add_index'],
-  refine min_le_min _ _,
-  { simp, split_ifs, { exact ha _, }, exact rfl.le, },
-  { simp, split_ifs, { exact hb _, }, exact rfl.le, },
-end
-
-lemma Stream.add_reduced [has_zero α] [has_add α] {a : Stream ι α} {b : Stream ι α}
-  (ha : a.reduced) (hb : b.reduced) : (a + b).reduced :=
-begin
-  rintros ⟨x, y⟩ hv hr,
-  rcases hr with ⟨h, hr⟩|⟨h, hr⟩;
-  dsimp at hr h ⊢,
-  { simp [h, (show min (a.index' x) (b.index' y) = _, from min_eq_left (prod.lex.fst_le_of_le h))],
-    apply ne_min_of_ne_and_ne, { exact ha _ hr, },
-    split_ifs with H,
-    { obtain ⟨h₁, h₂⟩ : a.index' x = b.index' y ∧ (a.ready x ↔ b.ready y),
-      { simpa [Stream.to_order] using (antisymm h H), },
-      rw h₁, exact hb _ (by rwa ← h₂), },
-    exact ne_of_lt (prod.lex.fst_lt_of_lt_of_le (lt_of_le_not_le h H) (by simp [hr])), },
-  { simp [h, (show min (a.index' x) (b.index' y) = _, from min_eq_right (prod.lex.fst_le_of_le h))],
-    apply ne_min_of_ne_and_ne, swap, { exact hb _ hr, },
-    split_ifs with H,
-    { obtain ⟨h₁, h₂⟩ : a.index' x = b.index' y ∧ (a.ready x ↔ b.ready y),
-      { simpa [Stream.to_order] using (antisymm H h), },
-      rw ← h₁, exact ha _ (by rwa h₂), },
-    exact ne_of_lt (prod.lex.fst_lt_of_lt_of_le (lt_of_le_not_le h H) (by simp [hr])), },
-end
-
-instance StreamExec.AddZeroEval [add_comm_monoid α] : AddZeroEval (StreamExec ι α) ι α :=
-{ hadd := StreamExec.add_spec,
-  hzero := StreamExec.zero_eval }
-
-lemma add_value_eval {ι α ι' α' : Type*} [linear_order ι] [add_comm_monoid α'] [AddZeroEval α ι' α'] 
-  (a b : StreamExec ι α) :
-  (Eval.eval <$₂> (a + b)) = (Eval.eval <$₂> a) + (Eval.eval <$₂> b) :=
-begin
-  ext; solve_refl,
-  simp [apply_ite Eval.eval],
-  congr; rw [Stream.bimap_value'_apply]; simp,
-end
-
-instance {ι α ι' α' : Type*} [linear_order ι] [add_comm_monoid α'] [AddZeroEval α ι' α'] :
-  AddZeroEval (StreamExec ι α) ι (ι' →₀ α') :=
-{ hadd := λ x y, by simp [Eval.eval, add_value_eval],
-  hzero := StreamExec.zero_eval }
-
-instance {ι : Type} {α : Type*} [linear_order ι] [has_zero α] [has_add α] : has_add (SimpleStream ι α) := ⟨λ a b,
-{ simple :=
-  { monotonic := Stream.add_monotonic a.monotonic b.monotonic,
-    reduced := Stream.add_reduced a.reduced b.reduced },
-  ..(@has_add.add (StreamExec ι α) _ a b) }⟩
-
-instance SimpleStream.AddZeroEvalBase [add_comm_monoid α] : AddZeroEval (SimpleStream ι α) ι α :=
-{ hadd := λ x y, by exact AddZeroEval.hadd (↑x : StreamExec _ _) (↑y : StreamExec _ _),
-  hzero := SimpleStream.zero_eval }
-
-instance SimpleStream.AddZeroEval {ι α ι' α' : Type*} [linear_order ι] [add_comm_monoid α'] [AddZeroEval α ι' α'] :
-  AddZeroEval (SimpleStream ι α) ι (ι' →₀ α') :=
-{ hadd := λ x y, by exact AddZeroEval.hadd (↑x : StreamExec _ _) (↑y : StreamExec _ _),
-  hzero := SimpleStream.zero_eval }
 
 
